src/Pyrosome/Compilers/ClosedCompilers.v
@@ -26,307 +26,257 @@ Section WithVar.
   Notation sort := (@sort V).
   Notation lang := (@lang V).
 
-  Section WithLangAndCtx.
-    Context (l : lang)
-      (c : ctx)
-      {CM : ClosedModel}
-      {CMok : ClosedModel_ok l c}.
+  Section WithTarget.
+    Context {tgt_term tgt_sort : Type}
+      {tgt_pre : @PreModel V tgt_term tgt_sort}
+      {tgt_term_default : WithDefault tgt_term}
+      {tgt_sort_default : WithDefault tgt_sort}.
 
-    (* --- Prop-valued evaluation of a proof tree into the ClosedModel.
-       This is Gluing/Eval.v's [eval] ported from the Type-valued CutTModel to
-       the Prop-valued ClosedModel; because [pf] is cut-free it is a direct fold,
-       one constructor per ClosedModel_ok operation, with no substitution case. *)
-    Local Notation Pp p :=
-      ((forall t1 t2, check_sort_proof l c p = Some (t1, t2) -> ceq_sort (ClosedModel:=CM) t1 t2)
-       /\ (forall t e1 e2, check_proof l c p = Some (e1, e2, t) -> ceq_term (ClosedModel:=CM) t e1 e2)).
+    (* --- From the per-rule inductive [preserving_closed_compiler_ext] to the
+       per-rule obligation for a named rule, phrased in the target model [CM] on
+       the compiled syntax.  These four "lookup" lemmas are the source of the
+       congruence / axiom-instance facts that [eval] folds into the model. *)
+    Section ExtLookups.
+      Context (cmp : closed_compiler V tgt_term tgt_sort)
+        (CM : @ClosedModel V tgt_term tgt_sort).
 
-    Lemma eval_args s
-      : fold_right (fun p => and (Pp p)) True s ->
-        forall c' lhs rhs,
-          check_args_proof (check_proof l c) s c' = Some (lhs, rhs) ->
-          ceq_args (CM:=CM) c' lhs rhs.
-    Proof.
-      induction s as [| p s IHs]; intros IH c' lhs rhs Hc.
-      - destruct c'; cbn in Hc; try discriminate.
-        safe_invert Hc. constructor.
-      - destruct IH as [Pp_p IH_s].
-        destruct c' as [| [name t] c'']; cbn in Hc; try discriminate.
-        destruct (check_args_proof (check_proof l c) s c'') as [[lhs0 rhs0] |] eqn:Hargs;
-          cbn in Hc; try discriminate.
-        destruct (check_proof l c p) as [[[e1 e2] t'] |] eqn:Hp;
-          cbn in Hc; try discriminate.
-        destruct (eqb t[/with_names_from c'' rhs0/] t') eqn:Heqb;
-          cbn in Hc; try discriminate.
-        safe_invert Hc.
-        assert (t[/with_names_from c'' rhs0/] = t') as Heq.
-        { apply (proj1 (eqb_prop_iff _ _ _)); rewrite Heqb; exact I. }
-        econstructor.
-        + eapply IHs; eauto.
-        + rewrite Heq. eapply (proj2 Pp_p); eauto.
-    Qed.
-
-    Theorem eval p : Pp p.
-    Proof.
-      induction p; split; intros; cbn in *;
-        repeat (lazymatch goal with
-                | [ HH : context [ match ?x with _ => _ end ] |- _ ] =>
-                    destruct x eqn:?
-                end; try discriminate);
-        try discriminate;
-        repeat (lazymatch goal with
-                | [ HH : Some _ = Some _ |- _ ] => safe_invert HH
-                | [ HH : _ /\ _ |- _ ] => destruct HH
-                | [ HH : named_list_lookup_err _ _ = Some _ |- _ ] => symmetry in HH
-                | [ HH : eqb ?a ?b = true |- _ ] =>
-                    let Heq := fresh "Heq" in
-                    assert (a = b) as Heq
-                      by (apply (proj1 (eqb_prop_iff _ _ _)); rewrite HH; exact I);
-                    clear HH; try subst a; try subst b
-                end);
-        eauto 8 using cterm_var, cterm_cong, cterm_by, cterm_trans, cterm_sym,
-                      cterm_conv, csort_cong, csort_by, csort_trans, csort_sym,
-                      eval_args with utils.
-    Qed.
-
-    Definition eval_sort p t1 t2
-      (H : check_sort_proof l c p = Some (t1, t2)) : ceq_sort (ClosedModel:=CM) t1 t2 :=
-      proj1 (eval p) t1 t2 H.
-
-    Definition eval_term p t e1 e2
-      (H : check_proof l c p = Some (e1, e2, t)) : ceq_term (ClosedModel:=CM) t e1 e2 :=
-      proj2 (eval p) t e1 e2 H.
-
-    Section Soundness.
-      Context (wfl : wf_lang l)
-        (wfc : wf_ctx (Model := core_model l) c).
-
-      (* A [ClosedModel_ok] is complete for the judgemental equalities: reuse
-         tree-proof completeness (CutModelSound) then evaluate the tree. *)
-      Theorem closed_model_sound_term t e1 e2
-        : eq_term l c t e1 e2 -> ceq_term (ClosedModel:=CM) t e1 e2.
+      Lemma pcce_term_rule_lookup
+        : forall l, preserving_closed_compiler_ext cmp CM l ->
+          forall n c' args t, In (n, term_rule c' args t) l ->
+          forall s1 s2, ceq_args (CM := compile_model cmp CM) c' s1 s2 ->
+            ceq_term (ClosedModel := CM) (compile_sort cmp (t [/with_names_from c' s2/]))
+              (compile cmp (con n s1)) (compile cmp (con n s2)).
       Proof.
-        intro H.
-        destruct (CutModelSound.tree_complete_term wfl wfc H) as [p Hp].
-        eapply eval_term; eauto.
+        intros l H.
+        induction H as
+          [ | l n c' args Hpre IH Hob
+            | l n c' args t Hpre IH Hob
+            | l n c' t1 t2 Hpre IH Hob
+            | l n c' e1 e2 t Hpre IH Hob ];
+          intros nn cc aa tt Hin s1 s2 Hargs.
+        - destruct Hin.
+        - destruct Hin as [Heq | Hin]; [ inversion Heq | ]; eapply IH; eauto.
+        - destruct Hin as [Heq | Hin];
+            [ inversion Heq; subst; eapply Hob; eauto | eapply IH; eauto ].
+        - destruct Hin as [Heq | Hin]; [ inversion Heq | ]; eapply IH; eauto.
+        - destruct Hin as [Heq | Hin]; [ inversion Heq | ]; eapply IH; eauto.
       Qed.
 
-      Theorem closed_model_sound_sort t1 t2
-        : eq_sort l c t1 t2 -> ceq_sort (ClosedModel:=CM) t1 t2.
+      Lemma pcce_sort_rule_lookup
+        : forall l, preserving_closed_compiler_ext cmp CM l ->
+          forall n c' args, In (n, sort_rule c' args) l ->
+          forall s1 s2, ceq_args (CM := compile_model cmp CM) c' s1 s2 ->
+            ceq_sort (ClosedModel := CM)
+              (compile_sort cmp (scon n s1)) (compile_sort cmp (scon n s2)).
       Proof.
-        intro H.
-        destruct (proj1 (CutModelSound.tree_complete wfl wfc) _ _ H) as [p Hp].
-        eapply eval_sort; eauto.
+        intros l H.
+        induction H as
+          [ | l n c' args Hpre IH Hob
+            | l n c' args t Hpre IH Hob
+            | l n c' t1 t2 Hpre IH Hob
+            | l n c' e1 e2 t Hpre IH Hob ];
+          intros nn cc aa Hin s1 s2 Hargs.
+        - destruct Hin.
+        - destruct Hin as [Heq | Hin];
+            [ inversion Heq; subst; eapply Hob; eauto | eapply IH; eauto ].
+        - destruct Hin as [Heq | Hin]; [ inversion Heq | ]; eapply IH; eauto.
+        - destruct Hin as [Heq | Hin]; [ inversion Heq | ]; eapply IH; eauto.
+        - destruct Hin as [Heq | Hin]; [ inversion Heq | ]; eapply IH; eauto.
       Qed.
 
-    End Soundness.
+      Lemma pcce_sort_eq_lookup
+        : forall l, preserving_closed_compiler_ext cmp CM l ->
+          forall n c' t1 t2, In (n, sort_eq_rule c' t1 t2) l ->
+          forall s1 s2, ceq_args (CM := compile_model cmp CM) c' s1 s2 ->
+            ceq_sort (ClosedModel := CM)
+              (compile_sort cmp (t1 [/with_names_from c' s1/]))
+              (compile_sort cmp (t2 [/with_names_from c' s2/])).
+      Proof.
+        intros l H.
+        induction H as
+          [ | l n c' args Hpre IH Hob
+            | l n c' args t Hpre IH Hob
+            | l n c' t1 t2 Hpre IH Hob
+            | l n c' e1 e2 t Hpre IH Hob ];
+          intros nn cc tt1 tt2 Hin s1 s2 Hargs.
+        - destruct Hin.
+        - destruct Hin as [Heq | Hin]; [ inversion Heq | ]; eapply IH; eauto.
+        - destruct Hin as [Heq | Hin]; [ inversion Heq | ]; eapply IH; eauto.
+        - destruct Hin as [Heq | Hin];
+            [ inversion Heq; subst; eapply Hob; eauto | eapply IH; eauto ].
+        - destruct Hin as [Heq | Hin]; [ inversion Heq | ]; eapply IH; eauto.
+      Qed.
 
-  End WithLangAndCtx.
+      Lemma pcce_term_eq_lookup
+        : forall l, preserving_closed_compiler_ext cmp CM l ->
+          forall n c' e1 e2 t, In (n, term_eq_rule c' e1 e2 t) l ->
+          forall s1 s2, ceq_args (CM := compile_model cmp CM) c' s1 s2 ->
+            ceq_term (ClosedModel := CM) (compile_sort cmp (t [/with_names_from c' s2/]))
+              (compile cmp (e1 [/with_names_from c' s1/]))
+              (compile cmp (e2 [/with_names_from c' s2/])).
+      Proof.
+        intros l H.
+        induction H as
+          [ | l n c' args Hpre IH Hob
+            | l n c' args t Hpre IH Hob
+            | l n c' t1 t2 Hpre IH Hob
+            | l n c' ee1 ee2 t Hpre IH Hob ];
+          intros nn cc ff1 ff2 tt Hin s1 s2 Hargs.
+        - destruct Hin.
+        - destruct Hin as [Heq | Hin]; [ inversion Heq | ]; eapply IH; eauto.
+        - destruct Hin as [Heq | Hin]; [ inversion Heq | ]; eapply IH; eauto.
+        - destruct Hin as [Heq | Hin]; [ inversion Heq | ]; eapply IH; eauto.
+        - destruct Hin as [Heq | Hin];
+            [ inversion Heq; subst; eapply Hob; eauto | eapply IH; eauto ].
+      Qed.
 
-  (* --- From the per-rule inductive [preserving_closed_compiler_ext] to the
-     semantic [preserving_closed_compiler] (i.e. the pullback is a
-     [ClosedModel_ok]).  The four "lookup" lemmas turn the derivation into the
-     obligation for a named rule; the theorem then assembles the record,
-     discharging the variable case and the structural (trans/sym/conv) laws
-     directly from the *target* model's [ClosedModel_ok] -- so those are never
-     obligations for the compiler author. *)
-  Section ExtSoundness.
-    Context (cmp : closed_compiler V) (CM : @ClosedModel V).
+    End ExtLookups.
 
-    Lemma pcce_term_rule_lookup
-      : forall l, preserving_closed_compiler_ext cmp CM l ->
-        forall n c' args t, In (n, term_rule c' args t) l ->
-        forall s1 s2, ceq_args (CM := compile_model cmp CM) c' s1 s2 ->
-          ceq_term (ClosedModel := CM) (compile_sort cmp (t [/with_names_from c' s2/]))
-            (compile cmp (con n s1)) (compile cmp (con n s2)).
-    Proof.
-      intros l H.
-      induction H as
-        [ | l n c' args Hpre IH Hob
-          | l n c' args t Hpre IH Hob
-          | l n c' t1 t2 Hpre IH Hob
-          | l n c' e1 e2 t Hpre IH Hob ];
-        intros nn cc aa tt Hin s1 s2 Hargs.
-      - destruct Hin.
-      - destruct Hin as [Heq | Hin]; [ inversion Heq | ]; eapply IH; eauto.
-      - destruct Hin as [Heq | Hin];
-          [ inversion Heq; subst; eapply Hob; eauto | eapply IH; eauto ].
-      - destruct Hin as [Heq | Hin]; [ inversion Heq | ]; eapply IH; eauto.
-      - destruct Hin as [Heq | Hin]; [ inversion Heq | ]; eapply IH; eauto.
-    Qed.
+    Section Eval.
+      Context (l : lang)
+        (cmp : closed_compiler V tgt_term tgt_sort)
+        (CM : @ClosedModel V tgt_term tgt_sort)
+        (CMok : ClosedModel_ok CM)
+        (Hext : preserving_closed_compiler_ext cmp CM l).
 
-    Lemma pcce_sort_rule_lookup
-      : forall l, preserving_closed_compiler_ext cmp CM l ->
-        forall n c' args, In (n, sort_rule c' args) l ->
-        forall s1 s2, ceq_args (CM := compile_model cmp CM) c' s1 s2 ->
-          ceq_sort (ClosedModel := CM)
-            (compile_sort cmp (scon n s1)) (compile_sort cmp (scon n s2)).
-    Proof.
-      intros l H.
-      induction H as
-        [ | l n c' args Hpre IH Hob
-          | l n c' args t Hpre IH Hob
-          | l n c' t1 t2 Hpre IH Hob
-          | l n c' e1 e2 t Hpre IH Hob ];
-        intros nn cc aa Hin s1 s2 Hargs.
-      - destruct Hin.
-      - destruct Hin as [Heq | Hin];
-          [ inversion Heq; subst; eapply Hob; eauto | eapply IH; eauto ].
-      - destruct Hin as [Heq | Hin]; [ inversion Heq | ]; eapply IH; eauto.
-      - destruct Hin as [Heq | Hin]; [ inversion Heq | ]; eapply IH; eauto.
-      - destruct Hin as [Heq | Hin]; [ inversion Heq | ]; eapply IH; eauto.
-    Qed.
+      (* The pullback of the target [CM] along [compile]; a [ClosedModel] over the
+         source syntax whose judgments are exactly the preservation conclusions.
+         Its judgments unfold to [CM]'s at the compiled syntax, so the fold below
+         discharges them with [CM]'s own structural laws ([CMok]) and the per-rule
+         congruence/axiom facts ([pcce_*_lookup], from [Hext]) directly. *)
+      Local Notation M := (compile_model cmp CM).
 
-    Lemma pcce_sort_eq_lookup
-      : forall l, preserving_closed_compiler_ext cmp CM l ->
-        forall n c' t1 t2, In (n, sort_eq_rule c' t1 t2) l ->
-        forall s1 s2, ceq_args (CM := compile_model cmp CM) c' s1 s2 ->
-          ceq_sort (ClosedModel := CM)
-            (compile_sort cmp (t1 [/with_names_from c' s1/]))
-            (compile_sort cmp (t2 [/with_names_from c' s2/])).
-    Proof.
-      intros l H.
-      induction H as
-        [ | l n c' args Hpre IH Hob
-          | l n c' args t Hpre IH Hob
-          | l n c' t1 t2 Hpre IH Hob
-          | l n c' e1 e2 t Hpre IH Hob ];
-        intros nn cc tt1 tt2 Hin s1 s2 Hargs.
-      - destruct Hin.
-      - destruct Hin as [Heq | Hin]; [ inversion Heq | ]; eapply IH; eauto.
-      - destruct Hin as [Heq | Hin]; [ inversion Heq | ]; eapply IH; eauto.
-      - destruct Hin as [Heq | Hin];
-          [ inversion Heq; subst; eapply Hob; eauto | eapply IH; eauto ].
-      - destruct Hin as [Heq | Hin]; [ inversion Heq | ]; eapply IH; eauto.
-    Qed.
+      (* The target model's structural laws, as plain references (so they can be
+         named in [eauto ... using] below). *)
+      Let ct_trans := CMok.(cterm_trans).
+      Let ct_sym := CMok.(cterm_sym).
+      Let ct_conv := CMok.(cterm_conv).
+      Let cs_trans := CMok.(csort_trans).
+      Let cs_sym := CMok.(csort_sym).
 
-    Lemma pcce_term_eq_lookup
-      : forall l, preserving_closed_compiler_ext cmp CM l ->
-        forall n c' e1 e2 t, In (n, term_eq_rule c' e1 e2 t) l ->
-        forall s1 s2, ceq_args (CM := compile_model cmp CM) c' s1 s2 ->
-          ceq_term (ClosedModel := CM) (compile_sort cmp (t [/with_names_from c' s2/]))
-            (compile cmp (e1 [/with_names_from c' s1/]))
-            (compile cmp (e2 [/with_names_from c' s2/])).
-    Proof.
-      intros l H.
-      induction H as
-        [ | l n c' args Hpre IH Hob
-          | l n c' args t Hpre IH Hob
-          | l n c' t1 t2 Hpre IH Hob
-          | l n c' ee1 ee2 t Hpre IH Hob ];
-        intros nn cc ff1 ff2 tt Hin s1 s2 Hargs.
-      - destruct Hin.
-      - destruct Hin as [Heq | Hin]; [ inversion Heq | ]; eapply IH; eauto.
-      - destruct Hin as [Heq | Hin]; [ inversion Heq | ]; eapply IH; eauto.
-      - destruct Hin as [Heq | Hin]; [ inversion Heq | ]; eapply IH; eauto.
-      - destruct Hin as [Heq | Hin];
-          [ inversion Heq; subst; eapply Hob; eauto | eapply IH; eauto ].
-    Qed.
+      (* --- Prop-valued evaluation of a proof tree into the pullback model [M].
+         This is Gluing/Eval.v's [eval] ported to the Prop-valued, closed
+         setting: the ambient context is empty (so the [pvar] case is vacuous). *)
+      Local Notation Pp p :=
+        ((forall t1 t2, check_sort_proof l [] p = Some (t1, t2) -> ceq_sort (ClosedModel:=M) t1 t2)
+         /\ (forall t e1 e2, check_proof l [] p = Some (e1, e2, t) -> ceq_term (ClosedModel:=M) t e1 e2)).
 
-    (* The ext inductive yields the pullback [ClosedModel_ok].  The target
-       [ClosedModel_ok] is needed only at ambient context [compile_ctx cmp c] and
-       only for its variable rule and its equational structural laws. *)
-    Theorem preserving_closed_compiler_ext_sound
-      (l : lang) (c : ctx) (l_tgt : lang)
-      (CMok : ClosedModel_ok l_tgt (compile_ctx cmp c))
-      (Hext : preserving_closed_compiler_ext cmp CM l)
-      : preserving_closed_compiler cmp l c CM.
-    Proof.
-      unfold preserving_closed_compiler.
-      unshelve econstructor; cbn [compile_model ceq_sort ceq_term].
-      - (* cterm_var *)
-        intros n t Hin.
-        change (compile cmp (var n)) with (var n).
-        apply CMok.(cterm_var).
-        apply in_named_map; exact Hin.
-      - (* cterm_cong *)
-        intros c' name args t s1 s2 Hin Hargs.
-        eapply pcce_term_rule_lookup; eauto.
-      - (* cterm_by *)
-        intros c' name e1 e2 t s1 s2 Hin Hargs.
-        eapply pcce_term_eq_lookup; eauto.
-      - (* cterm_trans *)
-        intros t e1 e12 e2 H1 H2; eapply CMok.(cterm_trans); eauto.
-      - (* cterm_sym *)
-        intros t e1 e2 H1; eapply CMok.(cterm_sym); eauto.
-      - (* cterm_conv *)
-        intros t1 t2 e1 e2 H1 H2; eapply CMok.(cterm_conv); eauto.
-      - (* csort_cong *)
-        intros c' name args s1 s2 Hin Hargs.
-        eapply pcce_sort_rule_lookup; eauto.
-      - (* csort_by *)
-        intros c' name t1 t2 s1 s2 Hin Hargs.
-        eapply pcce_sort_eq_lookup; eauto.
-      - (* csort_trans *)
-        intros t1 t12 t2 H1 H2; eapply CMok.(csort_trans); eauto.
-      - (* csort_sym *)
-        intros t1 t2 H1; eapply CMok.(csort_sym); eauto.
-    Qed.
+      Lemma eval_args s
+        : fold_right (fun p => and (Pp p)) True s ->
+          forall c' lhs rhs,
+            check_args_proof (check_proof l []) s c' = Some (lhs, rhs) ->
+            ceq_args (CM:=M) c' lhs rhs.
+      Proof.
+        induction s as [| p s IHs]; intros IH c' lhs rhs Hc.
+        - destruct c'; cbn in Hc; try discriminate.
+          safe_invert Hc. constructor.
+        - destruct IH as [Pp_p IH_s].
+          destruct c' as [| [name t] c'']; cbn in Hc; try discriminate.
+          destruct (check_args_proof (check_proof l []) s c'') as [[lhs0 rhs0] |] eqn:Hargs;
+            cbn in Hc; try discriminate.
+          destruct (check_proof l [] p) as [[[e1 e2] t'] |] eqn:Hp;
+            cbn in Hc; try discriminate.
+          destruct (eqb t[/with_names_from c'' rhs0/] t') eqn:Heqb;
+            cbn in Hc; try discriminate.
+          safe_invert Hc.
+          assert (t[/with_names_from c'' rhs0/] = t') as Heq.
+          { apply (proj1 (eqb_prop_iff _ _ _)); rewrite Heqb; exact I. }
+          econstructor.
+          + eapply IHs; eauto.
+          + assert (Hct : ceq_term (ClosedModel:=M) t' e1 e2)
+              by (eapply (proj2 Pp_p); reflexivity).
+            rewrite <- Heq in Hct.
+            exact Hct.
+      Qed.
 
-  End ExtSoundness.
+      Theorem eval p : Pp p.
+      Proof.
+        induction p; split; intros; cbn in *;
+          repeat (lazymatch goal with
+                  | [ HH : context [ match ?x with _ => _ end ] |- _ ] =>
+                      destruct x eqn:?
+                  end; try discriminate);
+          try discriminate;
+          repeat (lazymatch goal with
+                  | [ HH : Some _ = Some _ |- _ ] => safe_invert HH
+                  | [ HH : _ /\ _ |- _ ] => destruct HH
+                  | [ HH : named_list_lookup_err _ _ = Some _ |- _ ] => symmetry in HH
+                  | [ HH : eqb ?a ?b = true |- _ ] =>
+                      let Heq := fresh "Heq" in
+                      assert (a = b) as Heq
+                        by (apply (proj1 (eqb_prop_iff _ _ _)); rewrite HH; exact I);
+                      clear HH; try subst a; try subst b
+                  end);
+          eauto 8 using pcce_term_rule_lookup, pcce_term_eq_lookup,
+                        pcce_sort_rule_lookup, pcce_sort_eq_lookup,
+                        ct_trans, ct_sym, ct_conv, cs_trans, cs_sym,
+                        eval_args with utils.
+      Qed.
 
-  (* --- Main theorem: a preserving closed compiler preserves the judgemental
-     equalities.  Because preservation is *defined* as the pullback being a
-     ClosedModel_ok, each conclusion is a one-line instance of soundness above:
-     no substitution lemmas, no target Model_ok, no strengthening. *)
-  Section Preservation.
-    Context (l : lang)
-      (wfl : wf_lang l)
-      (c : ctx)
-      (wfc : wf_ctx (Model := core_model l) c)
-      (cmp : closed_compiler V)
-      (CM : ClosedModel)
-      (Hpres : preserving_closed_compiler cmp l c CM).
+      Definition eval_sort p t1 t2
+        (H : check_sort_proof l [] p = Some (t1, t2)) : ceq_sort (ClosedModel:=M) t1 t2 :=
+        proj1 (eval p) t1 t2 H.
 
-    Theorem closed_sort_eq_preserving t1 t2
-      : eq_sort l c t1 t2 ->
-        ceq_sort (ClosedModel:=CM) (compile_sort cmp t1) (compile_sort cmp t2).
-    Proof.
-      exact (@closed_model_sound_sort l c (compile_model cmp CM) Hpres wfl wfc t1 t2).
-    Qed.
+      Definition eval_term p t e1 e2
+        (H : check_proof l [] p = Some (e1, e2, t)) : ceq_term (ClosedModel:=M) t e1 e2 :=
+        proj2 (eval p) t e1 e2 H.
 
-    Theorem closed_term_eq_preserving t e1 e2
-      : eq_term l c t e1 e2 ->
-        ceq_term (ClosedModel:=CM) (compile_sort cmp t) (compile cmp e1) (compile cmp e2).
-    Proof.
-      exact (@closed_model_sound_term l c (compile_model cmp CM) Hpres wfl wfc t e1 e2).
-    Qed.
+      Section Soundness.
+        Context (wfl : wf_lang l).
 
-  End Preservation.
+        (* The pullback is complete for the judgemental equalities of closed
+           terms: reuse tree-proof completeness (CutModelSound) then evaluate the
+           tree.  The ambient context is empty, so [wf_ctx] is trivial. *)
+        Theorem closed_model_sound_term t e1 e2
+          : eq_term l [] t e1 e2 -> ceq_term (ClosedModel:=M) t e1 e2.
+        Proof.
+          intro H.
+          assert (wfc : wf_ctx (Model := core_model l) []) by constructor.
+          destruct (CutModelSound.tree_complete_term wfl wfc H) as [p Hp].
+          eapply eval_term; eauto.
+        Qed.
 
-  (* --- The compiler-author-facing entry point: from the per-rule inductive
-     [preserving_closed_compiler_ext] (one obligation per source rule) directly
-     to semantics preservation, given a well-formed target model at the compiled
-     ambient context.  No pullback record is ever exposed to the author. *)
-  Section PreservationFromExt.
-    Context (l : lang)
-      (wfl : wf_lang l)
-      (c : ctx)
-      (wfc : wf_ctx (Model := core_model l) c)
-      (l_tgt : lang)
-      (cmp : closed_compiler V)
-      (CM : ClosedModel)
-      (CMok : ClosedModel_ok l_tgt (compile_ctx cmp c))
-      (Hext : preserving_closed_compiler_ext cmp CM l).
+        Theorem closed_model_sound_sort t1 t2
+          : eq_sort l [] t1 t2 -> ceq_sort (ClosedModel:=M) t1 t2.
+        Proof.
+          intro H.
+          assert (wfc : wf_ctx (Model := core_model l) []) by constructor.
+          destruct (proj1 (CutModelSound.tree_complete wfl wfc) _ _ H) as [p Hp].
+          eapply eval_sort; eauto.
+        Qed.
 
-    Lemma preserving_from_ext : preserving_closed_compiler cmp l c CM.
-    Proof. eapply preserving_closed_compiler_ext_sound; eauto. Qed.
+      End Soundness.
 
-    Theorem closed_sort_eq_preserving_ext t1 t2
-      : eq_sort l c t1 t2 ->
-        ceq_sort (ClosedModel:=CM) (compile_sort cmp t1) (compile_sort cmp t2).
-    Proof.
-      exact (@closed_model_sound_sort l c (compile_model cmp CM) preserving_from_ext
-               wfl wfc t1 t2).
-    Qed.
+    End Eval.
 
-    Theorem closed_term_eq_preserving_ext t e1 e2
-      : eq_term l c t e1 e2 ->
-        ceq_term (ClosedModel:=CM) (compile_sort cmp t) (compile cmp e1) (compile cmp e2).
-    Proof.
-      exact (@closed_model_sound_term l c (compile_model cmp CM) preserving_from_ext
-               wfl wfc t e1 e2).
-    Qed.
+    (* --- Main theorem: a preserving closed compiler preserves the judgemental
+       equalities of closed terms/sorts.  Directly from the per-rule inductive
+       [preserving_closed_compiler_ext] and the target model's structural laws;
+       no substitution lemmas and no pullback record are exposed to the author. *)
+    Section Preservation.
+      Context (l : lang)
+        (wfl : wf_lang l)
+        (cmp : closed_compiler V tgt_term tgt_sort)
+        (CM : @ClosedModel V tgt_term tgt_sort)
+        (CMok : ClosedModel_ok CM)
+        (Hext : preserving_closed_compiler_ext cmp CM l).
 
-  End PreservationFromExt.
+      Theorem closed_sort_eq_preserving t1 t2
+        : eq_sort l [] t1 t2 ->
+          ceq_sort (ClosedModel:=CM) (compile_sort cmp t1) (compile_sort cmp t2).
+      Proof.
+        exact (@closed_model_sound_sort l cmp CM CMok Hext wfl t1 t2).
+      Qed.
+
+      Theorem closed_term_eq_preserving t e1 e2
+        : eq_term l [] t e1 e2 ->
+          ceq_term (ClosedModel:=CM) (compile_sort cmp t) (compile cmp e1) (compile cmp e2).
+      Proof.
+        exact (@closed_model_sound_term l cmp CM CMok Hext wfl t e1 e2).
+      Qed.
+
+    End Preservation.
+
+  End WithTarget.
 
 End WithVar.
